Broken version of strlen_apple

doc/examples/strlen/Apple/strlen.v
@@ -1,29 +1,211 @@
-From Coq Require Import String List ZArith.
+From Coq Require Import String List ZArith Lia.
 From compcert Require Import Coqlib Integers Floats AST Ctypes Cop Clight Clightdefs.
-Local Open Scope Z_scope.
+From compcert Require Import Maps Values ClightBigstep Events Memory.
+Open Scope Z_scope.
 
 Definition _s : ident := 54%positive.
 Definition _str : ident := 53%positive.
 Definition _strlen : ident := 55%positive.
-Definition _t'1 : ident := 57%positive.
+(* Definition _t : ident := 57%positive. *)
 
 Definition f_strlen := {|
   fn_return := tuint;
   fn_callconv := cc_default;
   fn_params := ((_str, (tptr tschar)) :: nil);
   fn_vars := nil;
-  fn_temps := ((_s, (tptr tschar)) :: (_t'1, tschar) :: nil);
+  fn_temps := ((_s, (tptr tschar)) :: nil);
   fn_body :=
 (Ssequence
   (Ssequence
     (Sset _s (Etempvar _str (tptr tschar)))
     (Sloop
-      (Ssequence
-        (Sset _t'1 (Ederef (Etempvar _s (tptr tschar)) tschar))
-        (Sifthenelse (Etempvar _t'1 tschar) Sskip Sbreak))
+    (* we don't need temporary variable _t *)
+    (Sifthenelse (Ederef (Etempvar _s (tptr tschar)) tschar) Sskip Sbreak)
       (Sset _s
+        (* add 1 to pointer _s *)
         (Ebinop Oadd (Etempvar _s (tptr tschar))
           (Econst_int (Int.repr 1) tint) (tptr tschar)))))
+  (* return result of substraction of _s with original pointer _str, 
+     with equals to 'len' *)
   (Sreturn (Some (Ebinop Osub (Etempvar _s (tptr tschar))
                    (Etempvar _str (tptr tschar)) tint))))
 |}.
+
+Definition f_strlen_loop := 
+    (Sloop
+    (* we don't need temporary variable _t *)
+    (Sifthenelse (Ederef (Etempvar _s (tptr tschar)) tschar) Sskip Sbreak)
+      (Sset _s
+        (* add 1 to pointer _s *)
+        (Ebinop Oadd (Etempvar _s (tptr tschar))
+          (Econst_int (Int.repr 1) tint) (tptr tschar)))).
+
+
+Inductive strlen_spec (m : mem) (b : block) (ofs : ptrofs) : nat -> Prop :=
+| LengthZero:
+    Mem.loadv Mint8signed m (Vptr b ofs) = Some (Vint Int.zero) ->
+    strlen_spec m b ofs 0
+| LengthSucc:
+    forall n c,
+    Z.of_nat (S n) < Int.modulus ->
+    Ptrofs.unsigned ofs + 1 < Ptrofs.modulus ->
+    Mem.loadv Mint8signed m (Vptr b ofs)  = Some (Vint c) ->
+    Int.eq c Int.zero = false ->
+    strlen_spec m b (Ptrofs.add ofs Ptrofs.one) n ->
+    strlen_spec m b ofs (S n).
+
+Definition nat_to_ofs (n : nat) := Ptrofs.repr (Z.of_nat n).
+
+Hint Resolve Ptrofs.mul_one Ptrofs.add_zero : ptrofs.
+
+Notation "x +* y" := (Ptrofs.add x y) (at level 80, right associativity).
+
+Lemma ofs_succ_l : forall ofs i,
+  Z.of_nat i < Int.modulus ->
+  ((ofs +* (nat_to_ofs i)) +* Ptrofs.one) =
+  (ofs +* (nat_to_ofs (S i))).
+Proof.
+  intros.
+  rewrite Ptrofs.add_assoc.
+  f_equal.
+  unfold nat_to_ofs, Ptrofs.add, Ptrofs.one, Ptrofs.mul.
+  rewrite Nat2Z.inj_succ.
+  rewrite Ptrofs.unsigned_repr_eq.
+  rewrite Zmod_small.
+  reflexivity.
+  replace Ptrofs.modulus with Int.modulus by reflexivity.
+  lia.
+Qed.
+
+Lemma ofs_succ_r : forall ofs i,
+  Z.of_nat i < Int.modulus ->
+  ((ofs +* Ptrofs.one) +* (nat_to_ofs i)) =
+  (ofs +* (nat_to_ofs (S i))).
+Proof.
+  intros.
+  rewrite <-ofs_succ_l by assumption.
+  rewrite Ptrofs.add_assoc, Ptrofs.add_assoc.
+  f_equal.
+  apply Ptrofs.add_commut.
+Qed.
+
+Lemma strlen_to_mem_0 :
+  forall len m b ofs,
+    strlen_spec m b ofs len ->
+    strlen_spec m b (ofs +* (nat_to_ofs len)) 0.
+Proof.
+  induction len.
+  all: intros.
+  - 
+    replace (nat_to_ofs 0) with Ptrofs.zero by reflexivity.
+    rewrite Ptrofs.add_zero.
+    assumption.
+  - 
+    inversion H.
+    rewrite <-ofs_succ_r by lia.
+    apply IHlen.
+    assumption.
+Qed.
+
+Lemma strlen_to_mem :
+  forall len m b ofs,
+    strlen_spec m b ofs len ->
+    forall i, (i < len)%nat ->
+         exists c, Int.eq c Int.zero = false /\
+           Mem.loadv Mint8signed m (Vptr b 
+             (ofs +* (nat_to_ofs i))) = Some (Vint c).
+Proof .
+  induction len. 
+  all: intros.
+  - lia.
+  - 
+    destruct i. 
+    all: inversion H.
+    * 
+      exists c.
+      split.
+      assumption.
+      rewrite Ptrofs.add_zero.
+      assumption.
+    * 
+      replace (ofs +* (nat_to_ofs (S i)))
+        with ((ofs +* Ptrofs.one) +* (nat_to_ofs i)).
+      apply IHlen.
+      assumption.
+      apply lt_S_n.
+      assumption.
+      rewrite ofs_succ_r by lia.
+      reflexivity.
+Qed.
+
+Lemma strlen_loop_correct_gen :
+  forall len i m b ofs ge e te,
+    strlen_spec m b ofs (len + i) ->   
+    exists t te',
+      te ! _str = Some (Vptr b ofs) ->
+      te ! _s = Some (Vptr b (ofs +* (nat_to_ofs i))) ->
+      exec_stmt ge e te m f_strlen_loop t te' m Out_normal
+      /\
+      te' ! _s = Some (Vptr b (ofs +* (nat_to_ofs (len + i)))).
+Proof.
+  induction len.
+  - 
+    intros.
+    repeat eexists.
+    repeat econstructor.
+    all: try eassumption.
+    *
+      apply strlen_to_mem_0 in H.
+      inversion H.
+      eassumption.
+    * reflexivity.
+    * repeat econstructor.
+  - 
+    intros.
+    assert (T : (i < S len + i)%nat) by lia.
+    pose proof strlen_to_mem _ _ _ _ H _ T as HM; clear T.
+    destruct HM as [c HM]; destruct HM as [HM1 HM2].
+    pose proof strlen_to_mem_0 _ _ _ _ H as HO.
+    replace (S len + i)%nat with (len + S i)%nat in * by lia.
+    (* starting env *)
+    remember ((PTree.set _s 
+               (Vptr b (Ptrofs.add 
+               (Ptrofs.add ofs (nat_to_ofs i)) Ptrofs.one)) te))
+      as Ite.
+    pose proof IHlen (S i) m b ofs ge e Ite H as IH.
+    clear IHlen.
+    destruct IH as [t' IH]. 
+    destruct IH as [te' IH].
+    repeat eexists.
+    destruct IH.
+    all: try subst.
+    rewrite PTree.gso.
+    all: try eassumption.
+    discriminate.
+    rewrite PTree.gss.
+    rewrite ofs_succ_l.
+    reflexivity.
+    inversion H.
+    all: try lia.
+    * 
+      eapply exec_Sloop_loop.
+      repeat econstructor.
+      eassumption.
+      eassumption.
+      reflexivity.
+      rewrite HM1.
+      repeat econstructor.
+      constructor.
+      repeat econstructor.
+      eassumption.
+      repeat econstructor.
+      fold f_strlen_loop.
+      replace (Ptrofs.mul (Ptrofs.repr (sizeof ge tschar)) (ptrofs_of_int Signed (Int.repr 1)))
+        with Ptrofs.one
+        by (auto with ptrofs).
+      eassumption.
+    * 
+      destruct IH.
+Qed.
+
+Close Scope Z.
